chore: adjust project structure
compatible with Coq 8.15.2
update hoare, redefine elem'as product type

theories/st_graph_nfa.v
@@ -18,7 +18,8 @@ Definition get_new_vertex' {T} : program (@state' T) Z := {|
     fun s1 n s2 =>
     s2.(max_v') = s1.(max_v') + 1 /\
     s2.(max_e') = s1.(max_e') /\
-    n = s2.(max_v');
+    n = s2.(max_v') /\
+    s2.(st_graph) = s1.(st_graph);
   err := fun s1 => False (* no error case *)
 |}.
 
@@ -27,7 +28,8 @@ Definition get_new_edge' {T} : program (@state' T) Z := {|
     fun s1 n s2 =>
     s2.(max_v') = s1.(max_v') /\
     s2.(max_e') = s1.(max_e') + 1 /\
-    n = s2.(max_v');
+    n = s2.(max_v') /\
+    s2.(st_graph) = s1.(st_graph);
   err := fun s1 => False (* no error case *)
 |}.
 
@@ -65,12 +67,17 @@ Definition pregraph_add_edge' {T} (e: Z) (s t: Z) (c : option T)
   (* error if edge exists *)
 |}.
 
+(* Definition pregraph_add_whole_vertex' {T}
+: program (@state' T) pg_nfa :=
+  v <- get_new_vertex' ;;
+  pregraph_add_vertex' v. *)
+
 Definition pregraph_add_whole_edge' {T} (s t: Z) (c: option T)
 : program state' pg_nfa :=
   e <- get_new_edge' ;;
   pregraph_add_edge' e s t c.
 
-Definition nfa_to_elem' {T} (sv ev: Z) : program (@state' T) elem' := {|
+(* Definition nfa_to_elem' {T} (sv ev: Z) : program (@state' T) elem' := {|
   nrm :=
     fun s1 E s2 =>
     s1 = s2 /\
@@ -82,63 +89,63 @@ Definition nfa_to_elem' {T} (sv ev: Z) : program (@state' T) elem' := {|
     fun s1 =>
     let g := s1.(st_graph) in
     ~ vvalid g.(pg) sv \/ ~ vvalid g.(pg) ev
-|}.
+|}. *)
 
 Fixpoint regexToNFA' {T} (r : reg_exp T)
 : program state' elem' :=
   match r with
   | EmptySet_r =>
     v1 <- get_new_vertex' ;;
-    v2 <- get_new_vertex' ;;
     pregraph_add_vertex' v1 ;;
+    v2 <- get_new_vertex' ;;
     pregraph_add_vertex' v2 ;;
-    nfa_to_elem' v1 v2
+    return (v1, v2)
 
   | EmptyStr_r =>
     v1 <- get_new_vertex' ;;
-    v2 <- get_new_vertex' ;;
     pregraph_add_vertex' v1 ;;
+    v2 <- get_new_vertex' ;;
     pregraph_add_vertex' v2 ;;
     pregraph_add_whole_edge' v1 v2 None ;;
-    nfa_to_elem' v1 v2
+    return (v1, v2)
 
   | Char_r t =>
     v1 <- get_new_vertex' ;;
-    v2 <- get_new_vertex' ;;
     pregraph_add_vertex' v1 ;;
+    v2 <- get_new_vertex' ;;
     pregraph_add_vertex' v2 ;;
     pregraph_add_whole_edge' v1 v2 (Some t) ;;
-    nfa_to_elem' v1 v2
+    return (v1, v2)
 
   | Concat_r r1 r2 =>
-    E1 <- regexToNFA' r1 ;;
-    E2 <- regexToNFA' r2 ;;
-    pregraph_add_whole_edge' E1.(endVertex') E2.(startVertex') epsilon ;;
-    nfa_to_elem' E1.(startVertex') E2.(endVertex')
+    '(sv1, ev1) <- regexToNFA' r1 ;;
+    '(sv2, ev2) <- regexToNFA' r2 ;;
+    pregraph_add_whole_edge' ev1 ev2 epsilon ;;
+    return (sv1, ev2)
 
   | Union_r r1 r2 =>
-    E1 <- regexToNFA' r1 ;;
-    E2 <- regexToNFA' r2 ;;
+    '(sv1, ev1) <- regexToNFA' r1 ;;
+    '(sv2, ev2) <- regexToNFA' r2 ;;
     v1 <- get_new_vertex' ;;
-    v2 <- get_new_vertex' ;;
     pregraph_add_vertex' v1 ;;
+    v2 <- get_new_vertex' ;;
     pregraph_add_vertex' v2 ;;
-    pregraph_add_whole_edge' v1 E1.(startVertex') epsilon ;;
-    pregraph_add_whole_edge' v1 E2.(startVertex') epsilon ;;
-    pregraph_add_whole_edge' E1.(endVertex') v2 epsilon ;;
-    pregraph_add_whole_edge' E2.(endVertex') v2 epsilon ;;
-    nfa_to_elem' E1.(startVertex') E2.(startVertex')
+    pregraph_add_whole_edge' v1 sv1 epsilon ;;
+    pregraph_add_whole_edge' v1 sv2 epsilon ;;
+    pregraph_add_whole_edge' ev1 v2 epsilon ;;
+    pregraph_add_whole_edge' ev2 v2 epsilon ;;
+    return (v1, v2)
 
   | Star_r r =>
-    E <- regexToNFA' r ;;
+    '(sv, ev) <- regexToNFA' r ;;
     v1 <- get_new_vertex' ;;
-    v2 <- get_new_vertex' ;;
     pregraph_add_vertex' v1 ;;
+    v2 <- get_new_vertex' ;;
     pregraph_add_vertex' v2 ;;
-    pregraph_add_whole_edge' v1 E.(endVertex') epsilon ;;
-    pregraph_add_whole_edge' E.(endVertex') v2 epsilon ;;
-    pregraph_add_whole_edge' E.(endVertex') E.(startVertex') epsilon ;;
-    nfa_to_elem' v1 v2
+    pregraph_add_whole_edge' v1 ev epsilon ;;
+    pregraph_add_whole_edge' ev v2 epsilon ;;
+    pregraph_add_whole_edge' ev sv epsilon ;;
+    return (v1, v2)
   end.
 
 (** recursion *)
