theories/hoare.v
@@ -3,6 +3,7 @@ Require Import Regex2NFA.theories.st_graph_nfa.
 Require Import Regex2NFA.theories.st_nograph_nfa.
 Require Import Regex2NFA.theories.regex.
 Require Import Coq.ZArith.ZArith.
+Require Import Lia.
 From StateMonad.monaderror Require Import monadEbasic monadEwhile monadesafe_lib monadEhoare.
 
 Import MonadwitherrDeno.
@@ -43,21 +44,73 @@ Lemma st_graph_inc {T: Type} :
 Proof.
 Admitted.
 
+Lemma get_new_vertex'_fact {T: Type} :
+  forall P,
+  Hoare P (@get_new_vertex' T) (
+                                fun n s =>
+                                  exists s',
+                                  n = s.(max_v') /\
+                                  s.(max_v') = s'.(max_v') + 1 /\
+                                  s.(max_e') = s'.(max_e') /\
+                                  s.(st_graph) = s'.(st_graph) /\
+                                  P s'
+                               ).
+Proof.
+unfold get_new_vertex', Hoare.
+split; intros.
+- eexists σ1.
+  destruct H0 as [?[?[?]]].
+  repeat split; auto.
+- eauto.
+Qed.
+
+Lemma pregraph_add_whole_vertex'_fact {T: Type} :
+  forall P,
+  Hoare P
+        (v <- @get_new_vertex' T ;; pregraph_add_vertex' v)
+        (
+          fun G s =>
+            exists s',
+            G = s.(st_graph) /\
+            s.(max_v') = s'.(max_v') + 1 /\
+            s.(max_e') = s'.(max_e') /\
+            G_add_vertex s'.(st_graph) s.(max_v') s.(st_graph) /\
+            P s'
+        ).
+Proof.
+intros. eapply Hoare_bind. 1 : { apply get_new_vertex'_fact. }
+intros. unfold pregraph_add_vertex', Hoare.
+split; intros.
+- destruct H as [?[?[?[?[]]]]].
+  destruct H0 as [?[?[?]]].
+  eexists x.
+  split. eauto.
+  split. lia.
+  split. lia.
+  split. rewrite <- H3. rewrite H0. rewrite <- H. eauto.
+  eauto.
+- destruct H as [?[?[?[?[]]]]].
+  destruct H0.
+  eauto.
+Qed.
+
 Lemma st_graph_refine {T: Type} :
   (** ∀ X, *)
   forall (r : reg_exp T) (G: @pg_nfa T) X,
-  Hoare ( fun s1 =>
+  Hoare (
+          fun s1 =>
             (** safeExec_X P_abs c_abs X *)
             (safeExec (fun s => s.(max_v) = s1.(max_v') /\ s.(max_e) = s1.(max_e'))
                       (regexToNFA r)
                       X) /\
             (*** P_con *)
-            s1.(st_graph) = G
-            (** G \forall v e, <= max_v max_e *)
+            s1.(st_graph) = G /\
+            (forall v, G.(pg).(vvalid) v -> v <= s1.(max_v')) /\
+            (forall e, G.(pg).(evalid) e -> e <= s1.(max_e'))
         )
         (regexToNFA' r) (** c_con *)
         ( 
-          fun el' s2 =>
+          fun '(sv, ev) s2 =>
             (** ∃ a, safeExec_X Q_abs(a) skip *)
             exists el, (safeExec (
                                    fun s => s.(max_v) = s2.(max_v') /\
@@ -66,13 +119,19 @@ Lemma st_graph_refine {T: Type} :
                                  (return el) (*? skip *)
                                  X
                        ) /\
+            (*? *)
+            (forall n, el.(graph).(pg).(vvalid) n -> n <= s2.(max_v')) /\
+            (forall n, el.(graph).(pg).(evalid) n -> n <= s2.(max_e')) /\
             (** Q_con(a) *)
-            let g := G.(pg) in
-              el'.(startVertex') = el.(startVertex) /\
-              el'.(endVertex') = el.(endVertex) /\
-              G_union_rel G el.(graph) s2.(st_graph) (** refinement *)
+            sv = el.(startVertex) /\
+            ev = el.(endVertex) /\
+            G_union_rel G el.(graph) s2.(st_graph) (** refinement *)
         ).
 Proof.
+induction r.
+- intros. simpl regexToNFA'.
+  intros. eapply Hoare_bind. 1 : { apply get_new_vertex'_fact. }
+  intros. eapply Hoare_bind.
 Admitted.
 
 Check safeExec.
