Makefile
@@ -1,8 +1,8 @@
-CURRENT_DIR=.
-SETS_DIR = ./sets
-FIXPOINT_DIR = ./fixedpoints
-MONAD_DIR = ./monadlib
-CERTIGRAPH_DIR = ./CertiGraph
+CURRENT_DIR = .
+SETS_DIR = sets
+FIXPOINT_DIR = fixedpoints
+MONAD_DIR = monadlib
+CERTIGRAPH_DIR = CertiGraph
 
 COQBIN=
 
@@ -12,17 +12,52 @@ COQC=$(COQBIN)coqc
 COQDEP=$(COQBIN)coqdep
 
 SETS_FLAG = -R $(SETS_DIR) SetsClass 
-FIXPOINT_FLAG = -R $(FIXPOINT_DIR) FP
-MONAD_FLAG = $(SETS_FLAG) $(FIXPOINT_FLAG) -R $(MONAD_DIR)/monadnrm StateMonad.monadnrm -R $(MONAD_DIR)/monaderror StateMonad.monaderror
+FIXPOINT_FLAG = $(SETS_FLAG) -R $(FIXPOINT_DIR) FP
+MONAD_FLAG = $(FIXPOINT_FLAG) -R $(MONAD_DIR)/monadnrm StateMonad.monadnrm -R $(MONAD_DIR)/monaderror StateMonad.monaderror
 CERTIGRAPH_FLAG = -R $(CERTIGRAPH_DIR) CertiGraph.lib
 
 DEP_FLAG = $(MONAD_FLAG) $(CERTIGRAPH_FLAG) -R lib Regex2NFA.lib -R theories Regex2NFA.theories
 
-CertiGraphlib_Files = \
+SETS_Files = \
+  SetsClass.v \
+  SetsClass_AxiomFree.v \
+  SetsDomain.v \
+  SetElement.v \
+  SetElementProperties.v \
+  RelsDomain.v \
+  SetProd.v \
+  SetsDomain_Classic.v
+
+SETS_FILES = \
+	$(SETS_Files:%.v=$(SETS_DIR)/%.v)
+
+FIXPOINT_Files = \
+  AllFramework.v \
+  Coqlib.v \
+  LiftConstructors.v \
+  PartialOrder_Setoid.v \
+  KnasterTarski.v \
+  BourbakiWitt.v \
+  SetsFixedpoints.v
+
+FIXPOINT_FILES = \
+	$(FIXPOINT_Files:%.v=$(FIXPOINT_DIR)/%.v)
+
+MonadNrm_Files = \
+	monadbasic.v safeexec_lib.v mergeExample.v
+
+MonadError_Files = \
+	monadEbasic.v monadEwhile.v monadesafe_lib.v monadEhoare.v
+  
+MONAD_FILES = \
+	$(MonadNrm_Files:%.v=$(MONAD_DIR)/monadnrm/%.v) \
+	$(MonadError_Files:%.v=$(MONAD_DIR)/monaderror/%.v) \
+
+CertiGraph_Files = \
 	Coqlib.v EquivDec_ext.v Ensembles_ext.v
 
 CERTIGRAPH_FILES = \
-	$(CertiGraphlib_Files:%.v=CertiGraph/%.v)
+	$(CertiGraph_Files:%.v=$(CERTIGRAPH_DIR)/%.v)
 
 Regex2NFAlib_Files = \
 	PreGraph.v
@@ -34,22 +69,36 @@ Regex2NFA_FILES = \
 	$(Regex2NFAlib_Files:%.v=lib/%.v) \
 	$(Regex2NFAtheories_Files:%.v=theories/%.v)
 
-FILES = $(CERTIGRAPH_FILES) $(Regex2NFA_FILES)
+FILES = \
+	$(SETS_FILES) \
+	$(FIXPOINT_FILES) \
+	$(MONAD_FILES) \
+	$(CERTIGRAPH_FILES) \
+	$(Regex2NFA_FILES)
 
-$(Regex2NFA_FILES:%.v=%.vo): %.vo: %.v
+$(SETS_FILES:%.v=%.vo): %.vo: %.v
 	@echo COQC $(<F)
-	@$(COQC) $(DEP_FLAG) $<
+	@$(COQC) $(SETS_FLAG) $<
+
+$(FIXPOINT_FILES:%.v=%.vo): %.vo: %.v
+	@echo COQC $(<F)
+	@$(COQC) $(FIXPOINT_FLAG) $<
+
+$(MONAD_FILES:%.v=%.vo): %.vo: %.v
+	@echo COQC $(<F)
+	@$(COQC) $(MONAD_FLAG) $<
 
 $(CERTIGRAPH_FILES:%.v=%.vo): %.vo: %.v
 	@echo COQC $(<F)
 	@$(COQC) $(CERTIGRAPH_FLAG) $<
 
-world:
-	$(MAKE) -C $(SETS_DIR)
-	$(MAKE) -C $(FIXPOINT_DIR)
-	$(MAKE) -C $(MONAD_DIR)
+$(Regex2NFA_FILES:%.v=%.vo): %.vo: %.v
+	@echo COQC $(<F)
+	@$(COQC) $(DEP_FLAG) $<
 
-all: $(FILES:%.v=%.vo)
+world: $(FILES:%.v=%.vo)
+
+all: world
 
 _CoqProject:
 	@echo $(DEP_FLAG) > _CoqProject
@@ -61,17 +110,14 @@ depend: $(FILES)
 	@$(COQDEP) $(DEP_FLAG) $(FILES) > .depend
 
 clean:
-	$(MAKE) -C $(SETS_DIR) clean
-	$(MAKE) -C $(FIXPOINT_DIR) clean
-	$(MAKE) -C $(MONAD_DIR) clean
 	@rm -f .lia.cache .nia.cache .depend _CoqProject
-	@rm -f lib/*.{vo,vos,vok,glob}
-	@rm -f theories/*.{vo,vos,vok,glob}
 	@rm -f sets/*.{vo,vos,vok,glob}
 	@rm -f fixedpoints/*.{vo,vos,vok,glob}
 	@rm -f monadlib/monadnrm/*.{vo,vos,vok,glob}
 	@rm -f monadlib/monaderror/*.{vo,vos,vok,glob}
 	@rm -f CertiGraph/*.{vo,vos,vok,glob}
+	@rm -f lib/*.{vo,vos,vok,glob}
+	@rm -f theories/*.{vo,vos,vok,glob}
 
 .DEFAULT_GOAL := all
 
